differentiability.v
@@ -1,0 +1,60 @@
+Require Import CoRN.algebra.CSetoids.
+Require Import CoRN.reals.CauchySeq.
+Require Import CoRN.ftc.MoreIntervals.
+
+Require Import SAMPL.reals.
+Require Import SAMPL.functions.
+
+(**
+* Definitions
+*)
+
+Section Differentiability_definitions.
+
+(**
+** Differentiability
+*)
+
+(**
+In this part, [I] is an interval $$\neq \emptyset$$ of $$\mathbb{R}, $$f : I \rightarrow \mathbb{R}$$.
+It's likely some of the definitions below already exist in the CoRN library (because we are using CoRN's [PartFunc]
+definition for partial functions. If it is the case, we prove the equivalence between our definitions and the
+CoRN's ones.
+*)
+
+Variable f : PartIR.
+Let I := Dom f.
+Section difference_quotient.
+
+(**
+We define the difference quotient of [f] as follows :
+$$\Delta_f (x_0, x) = \frac{f(x) - f(x_0)}{x - x_0}$$
+(N.B. : (\Delta_f (x_0, x) = \Delta_f (x, x_0)$$)
+*)
+
+Variable x0 : IR.
+Hypothesis H_x0 : I x0.
+Variable x : IR.
+Hypothesis H_x_I : I x.
+Hypothesis H_x_not_x0 : x[#]x0.
+
+Lemma x_x0_not_zero : x[-]x0 [#] [0].
+Proof. 
+    apply minus_ap_zero ; assumption.
+Admitted.
+
+Definition diff_quotient :=  (f x H_x_I [-] f x0 H_x0) [/] (x[-]x0) [//] x_x0_not_zero.
+
+End difference_quotient.
+
+Check diff_quotient.
+
+Lemma dq_pos_increasing_fun : (increasing_fun f) <-> (forall (x x0 : IR)(Hx : I x)(Hx0 : I x0), I x 
+     -> I x0 -> (diff_quotient x0 Hx0 x Hx) [>=] [0]).
+Proof.
+    unfold iff ; split.
+        intros. 
+
+End Differentiability_definitions.
+
+
